LambdaLab/Stlc/Named/Step/Basic.lean
@@ -10,7 +10,7 @@ substitution from `Basic.lean`.
 
 namespace LambdaLab.Stlc.Named
 
-inductive Step : Term → Term → Prop where
+inductive Step : (Term String) → (Term String) → Prop where
   | beta : Step (.app (.lam x τ body) v) (body.subst x v)
   | lam  : Step e e' → Step (.lam x τ e) (.lam x τ e')
   | appL : Step e₁ e₁' → Step (.app e₁ e₂) (.app e₁' e₂)
